{
 "cells": [
  {
   "cell_type": "markdown",
   "metadata": {},
   "source": [
    "1. Compute derivatives of functions:\n",
    "   * $y(x) = -3x+3$\n",
    "   * $y(x) = \\pi x + \\sin(1)$\n",
    "   * $y(x) = 4+\\sin(2)$\n",
    "   * $y(x) = 2x^3 - 3x^2 + 8x - 9$\n",
    "   * $y(x) = 6 x^{1/3}$\n",
    "   * $y(x) = \\sqrt{x}$\n",
    "   * $y(x) = \\cos(x) + \\sin(x)$\n",
    "   * $y(x) = 2\\sin(x) \\cos(x)$\n",
    "   * $y(x) = x\\sin(x)$\n",
    "   * $y(x) = (x+1)(x+1)$\n",
    "   * $y(x) = \\frac{x}{x+1}$\n",
    "   * $y(x) = (x+1)\\exp(x)$\n",
    "   * $y(x) = \\sin(x^2)$\n",
    "   * $y(x) = \\exp(-2x)$\n",
    "   * $y(x) = \\frac{1}{\\sin(x+1)}$\n",
    "   * $y(x) = \\sqrt{2x+1}$\n",
    "\n",
    "### Answers of Exercise #1\n",
    "\n",
    "1. **\\( y(x) = -3x + 3 \\):**\n",
    "   $$\n",
    "   y'(x) = -3\n",
    "   $$\n",
    "\n",
    "2. **\\( y(x) = \\pi x + \\sin(1) \\):**\n",
    "   - \\( \\sin(1) \\) is a constant, so its derivative is 0.\n",
    "   $$\n",
    "   y'(x) = \\pi\n",
    "   $$\n",
    "\n",
    "3. **\\( y(x) = 4 + \\sin(2) \\):**\n",
    "   - Both terms are constants, so:\n",
    "   $$\n",
    "   y'(x) = 0\n",
    "   $$\n",
    "\n",
    "4. **\\( y(x) = 2x^3 - 3x^2 + 8x - 9 \\):**\n",
    "   Using the power rule:\n",
    "   $$\n",
    "   y'(x) = 6x^2 - 6x + 8\n",
    "   $$\n",
    "\n",
    "5. **\\( y(x) = 6x^{1/3} \\):**\n",
    "   Using the power rule:\n",
    "   $$\n",
    "   y'(x) = 6 \\cdot \\frac{1}{3} x^{-2/3} = 2x^{-2/3}\n",
    "   $$\n",
    "\n",
    "6. **\\( y(x) = \\sqrt{x} \\):**\n",
    "   Rewrite \\( \\sqrt{x} \\) as \\( x^{1/2} \\), then use the power rule:\n",
    "   $$\n",
    "   y'(x) = \\frac{1}{2}x^{-1/2} = \\frac{1}{2\\sqrt{x}}\n",
    "   $$\n",
    "\n",
    "7. **\\( y(x) = \\cos(x) + \\sin(x) \\):**\n",
    "   Using the derivatives of trigonometric functions:\n",
    "   $$\n",
    "   y'(x) = -\\sin(x) + \\cos(x)\n",
    "   $$\n",
    "\n",
    "8. **\\( y(x) = 2\\sin(x)\\cos(x) \\):**\n",
    "   Use the product rule:\n",
    "   $$\n",
    "   y'(x) = 2\\cos^2(x) - 2\\sin^2(x)\n",
    "   $$\n",
    "   Alternatively, simplify using \\( \\sin(2x) \\):\n",
    "   $$\n",
    "   y'(x) = \\sin(2x)\n",
    "   $$\n",
    "\n",
    "9. **\\( y(x) = x\\sin(x) \\):**\n",
    "   Use the product rule:\n",
    "   $$\n",
    "   y'(x) = 1 \\cdot \\sin(x) + x \\cdot \\cos(x) = \\sin(x) + x\\cos(x)\n",
    "   $$\n",
    "\n",
    "10. **\\( y(x) = (x+1)(x+1) \\):**\n",
    "    Rewrite as \\( y(x) = (x+1)^2 \\) and use the chain rule:\n",
    "    $$\n",
    "    y'(x) = 2(x+1)\n",
    "    $$\n",
    "\n",
    "11. **\\( y(x) = \\frac{x}{x+1} \\):**\n",
    "    Use the quotient rule:\n",
    "    $$\n",
    "    y'(x) = \\frac{(1)(x+1) - (x)(1)}{(x+1)^2} = \\frac{1}{(x+1)^2}\n",
    "    $$\n",
    "\n",
    "12. **\\( y(x) = (x+1)\\exp(x) \\):**\n",
    "    Use the product rule:\n",
    "    $$\n",
    "    y'(x) = (1)(\\exp(x)) + (x+1)(\\exp(x)) = \\exp(x) + (x+1)\\exp(x) = (x+2)\\exp(x)\n",
    "    $$\n",
    "\n",
    "13. **\\( y(x) = \\sin(x^2) \\):**\n",
    "    Use the chain rule:\n",
    "    $$\n",
    "    y'(x) = \\cos(x^2) \\cdot 2x = 2x\\cos(x^2)\n",
    "    $$\n",
    "\n",
    "14. **\\( y(x) = \\exp(-2x) \\):**\n",
    "    Use the chain rule:\n",
    "    $$\n",
    "    y'(x) = \\exp(-2x) \\cdot (-2) = -2\\exp(-2x)\n",
    "    $$\n",
    "\n",
    "15. **\\( y(x) = \\frac{1}{\\sin(x+1)} \\):**\n",
    "    Rewrite as \\( y(x) = (\\sin(x+1))^{-1} \\) and use the chain rule:\n",
    "    $$\n",
    "    y'(x) = -\\frac{\\cos(x+1)}{\\sin^2(x+1)}\n",
    "    $$\n",
    "\n",
    "16. **\\( y(x) = \\sqrt{2x+1} \\):**\n",
    "    Rewrite as \\( y(x) = (2x+1)^{1/2} \\) and use the chain rule:\n",
    "    $$\n",
    "    y'(x) = \\frac{1}{2}(2x+1)^{-1/2} \\cdot 2 = \\frac{1}{\\sqrt{2x+1}}\n",
    "    $$"
   ]
  },
  {
   "cell_type": "markdown",
   "metadata": {},
   "source": [
    "2. Prove:\n",
    "   - $\\frac{d}{dx} (\\ln(\\sin(x))) = \\cot(x)$\n",
    "\n",
    "\n",
    "Start with the derivative of the natural logarithm:\n",
    "   $$\n",
    "   \\frac{d}{dx} (\\ln(\\sin(x))) = \\frac{1}{\\sin(x)} \\cdot \\frac{d}{dx}(\\sin(x))\n",
    "   $$\n",
    "\n",
    "The derivative of \\( \\sin(x) \\) is \\( \\cos(x) \\):\n",
    "   $$\n",
    "   \\frac{d}{dx} (\\ln(\\sin(x))) = \\frac{\\cos(x)}{\\sin(x)}\n",
    "   $$\n",
    "Simplify \\( \\frac{\\cos(x)}{\\sin(x)} \\) to \\( \\cot(x) \\):\n",
    "   $$\n",
    "   \\frac{d}{dx} (\\ln(\\sin(x))) = \\cot(x)\n",
    "   $$"
   ]
  },
  {
   "cell_type": "markdown",
   "metadata": {},
   "source": [
    "3. For $f(x) = \\cos(x)$, verify that $f''(x) = -f(x)$.\n",
    "\n",
    "### Answers of Exercise #3\n",
    "\n",
    "Compute the first derivative:\n",
    "   $$\n",
    "   f'(x) = \\frac{d}{dx} (\\cos(x)) = -\\sin(x)\n",
    "   $$\n",
    "Compute the second derivative:\n",
    "   $$\n",
    "   f''(x) = \\frac{d}{dx} (-\\sin(x)) = -\\cos(x)\n",
    "   $$\n",
    "Compare \\( f''(x) \\) with \\( -f(x) \\):\n",
    "   Since \\( f(x) = \\cos(x) \\), we find:\n",
    "   $$\n",
    "   f''(x) = -f(x)\n",
    "   $$"
   ]
  },
  {
   "cell_type": "markdown",
   "metadata": {},
   "source": [
    "4. Using de l'Hospital's Rule, find the improper limits:\n",
    "   - $\\displaystyle \\lim_{x\\to 0} \\frac{\\sin{x}}{x}$\n",
    "\n",
    "   - $\\displaystyle \\lim_{x\\to \\infty} \\frac{\\ln x}{x}$\n",
    "\n",
    "   - $\\displaystyle \\lim_{x\\to \\infty} \\frac{\\exp(x)}{x}$"
   ]
  },
  {
   "cell_type": "markdown",
   "metadata": {},
   "source": [
    "5. In physics, the position of a particle is given by $x(t) = 3t^2 - 6t + 1$. Find the velocity $V(t)=x'(t)$ and acceleration $a(t)=V'(t)=x''(t)$ of the particle at time $t = 2$."
   ]
  }
 ],
 "metadata": {
  "language_info": {
   "name": "python"
  }
 },
 "nbformat": 4,
 "nbformat_minor": 2
}
